stash

theories/BWT/BurrowsWheeler.v
@@ -1,4 +1,4 @@
-Require Import Coq.Lists.List.
+Require Coq.Lists.List.
 Require Import Coq.omega.Omega.
 Require Import Coq.Relations.Relation_Definitions.
 Require Import Coq.Classes.EquivDec.
@@ -15,368 +15,26 @@ Require Import BWT.Sorting.Ord.
 Require Import BWT.Repeat.
 Require Import BWT.Rots.
 Require Import BWT.Instances.
+Require Import BWT.Lib.
+Require Import BWT.Permutations.
+Require Import BWT.FindIx.
+Require Import BWT.Matrix.
+Require Import BWT.NonEmptyList.
 
 Import ListNotations.
 
 Open Scope program_scope.
 
-Lemma eq_map {A B : Type} (f g : A -> B) l :
-  (forall x, f x = g x) -> map f l = map g l.
-Proof.
-  intros HExt; induction l; try reflexivity.
-  simpl; rewrite HExt, IHl.
-  reflexivity.
-Qed.
+Section Transform.
+  Context {A : Type} `{O: Ord A} `{E : EqDec A eq}.
 
-Lemma map_map' {A B C : Type} : forall (f : A -> B) (g : B -> C) l,
-    map g (map f l) = map (g ∘ f) l.
-Proof.
-  intros.
-  rewrite map_map. apply eq_map.
-  reflexivity.
-Qed.
+  Definition bwp (l: list A) : list A :=
+    map last (sort (rots l)).
 
-Lemma Forall2_eq {A : Type} : forall x y : list A,
-    Forall2 eq x y <-> x = y.
-Proof.
-  split; intros.
-  - induction H.
-    + reflexivity.
-    + subst. f_equal.
-  - subst. induction y; constructor; auto.
-Qed.
-
-Lemma Forall2_map {A B : Type} (R : B -> B -> Prop) : forall (f : A -> B) (l l' : list A),
-    length l = length l' ->
-    Forall2 R (map f l) (map f l') <-> Forall2 (fun x y => R (f x) (f y)) l l'.
-Proof.
-  induction l; intros.
-  - simpl in H.
-    replace l' with (@nil A) by (symmetry; apply length_zero_iff_nil; auto).
-    split; constructor.
-  - destruct l' as [|a' l']; [inversion H|].
-    simpl; split; intros HImp; inversion HImp; subst; clear HImp; constructor; auto.
-    + apply IHl; auto.
-    + apply IHl; auto.
-Qed.
-
-Lemma Forall2_impl : forall (A B : Type) (P Q : A -> B -> Prop),
-    (forall a b, P a b -> Q a b) -> forall l l', Forall2 P l l' -> Forall2 Q l l'.
-Proof.
-  intros. induction H0; constructor; auto.
-Qed.
-
-Lemma map_injective {A B : Type} : forall (f : A -> B) l l',
-    (forall x y, f x = f y -> x = y) ->
-    map f l = map f l' -> l = l'.
-Proof.
-  intros f l l' HInj MapEq.
-  assert (length l = length l'). {
-    rewrite <- map_length with (f := f), MapEq, -> map_length.
-    easy.
-  }
-  assert (Forall2 (fun x y => f x = f y) l l'). {
-    apply Forall2_eq in MapEq.
-    apply (proj1 (Forall2_map eq f l l' H)) in MapEq.
-    apply MapEq.
-  }
-  apply Forall2_eq.
-  eapply Forall2_impl; [| apply H0].
-  cbv beta; intros. auto.
-Qed.
-
-Lemma map_forall_eq {A B : Type} : forall (l : list A) (f g : A -> B),
-    Forall (fun x => f x = g x) l -> map f l = map g l.
-Proof.
-  induction l; intros.
-  - reflexivity.
-  - inversion H; subst; clear H.
-    simpl. f_equal; auto.
-Qed.
-
-Section Permutations.
-  Context {A : Type} {P : A -> Prop} .
-  Variables l l' : list A.
-  Hypothesis HP : Permutation l l'.
-
-  Theorem Permutation_exists :
-    Exists P l -> Exists P l'.
-  Proof.
-    intros HE.
-    apply Exists_exists.
-    apply Exists_exists in HE; destruct HE as [x [HIn HPx]].
-    eauto using Permutation_in.
-  Defined.
-
-  Theorem Permutation_forall :
-    Forall P l -> Forall P l'.
-  Proof.
-    intros.
-    apply Forall_forall.
-    intros a HA.
-    apply Permutation_in with (l' := l) in HA; auto using Permutation_sym.
-    revert a HA.
-    apply Forall_forall.
-    auto.
-  Qed.
-End Permutations.
-
-Section SortRotations.
-  Context {A : Type} `{O : Ord A}.
-
-  Theorem foo : forall k l,
-sort (S k) (map rrot l) = (sort 1 ∘ map rrot) (sort k l) ->
-      @sort A O (S k) (map rrot l) = @sort A O 1 (map rrot (sort k l)).
-  Proof. unfold compose in *. easy. Qed.
-
-  Lemma sort_succ_k : forall k l,
-      sort (S k) l = sort 1 (map rrot (sort k (map lrot l))).
-  Proof.
-  Admitted.
-
-  Theorem sort_rrot_k : forall k l,
-    sort k (map (rep rrot k) l)= rep (sort 1 ∘ map rrot) k l.
-  Proof.
-  Admitted.
-
-  Lemma sort_succ_rrot : forall k (l : list (list A)),
-      @sort A O (S k) (map rrot l) = @sort A O 1 (map rrot (sort k l)).
-  Proof.
-    intros.
-    pose proof (sort_rrot_k (S k)) as E6.
-    simpl rep at 2 in E6.
-    specialize E6 with (l := map (rep lrot k) l).
-    rewrite <- sort_rrot_k in E6.
-    pose proof rep_inv_r (@lrot A) rrot l_r_rot_inverse as rep_inv.
-    do 2 rewrite map_map' in E6.
-    rewrite eq_map with (f := rep rrot (S k) ∘ rep lrot k) (g := rrot) in E6
-      by (intros; unfold compose;
-          rewrite rep_inv, Nat.sub_succ_l, Nat.sub_diag;
-          [reflexivity|apply Nat.le_refl|apply Nat.le_succ_diag_r]).
-    rewrite eq_map with (f := rep rrot k ∘ rep lrot k) (g := id)in E6
-      by (intros; unfold compose; rewrite rep_inv;
-          [rewrite Nat.sub_diag; reflexivity|apply Nat.le_refl]).
-    (* TODO For some reason hangs at the end *)
-    replace (sort 1 (map rrot (sort k l)))
-    with ((sort 1 ∘ map rrot) (sort k l)) by reflexivity.
-    rewrite map_id in E6.
-    apply E6.
-  Qed.
-
-End SortRotations.
-
-Section Cols.
-  Context {A : Type}.
-
-  Definition cols j := map (@firstn A j).
-
-  Context `{Ord A}.
-
-  Theorem cols_sort1 : forall k j l,
-      cols j (sort k l) = cols j (sort (Nat.min j k) l).
-  Admitted.
-
-  Theorem cols_sort2 : forall k j l,
-      cols j (sort k l) = sort (Nat.min j k) (cols j l).
-  Admitted.
-
-  Lemma cols_sort_lt : forall k j l,
-      j <= k -> cols j (sort k l) = sort j (cols j l).
-  Proof.
-    intros.
-    replace j with (Nat.min j k) at 2 by (apply Min.min_l; auto).
-    apply cols_sort2.
-  Qed.
-
-  Theorem cols_sort_perm : forall k j p l,
-      (forall l, Permutation l (p l)) -> cols j (sort k (p l)) = cols j (sort k l).
-  Admitted.
-
-  Theorem cols_sort_shift : forall k j l,
-      1 <= j <= k ->
-      cols j (sort k (rots l)) = sort 1 (cols j (map rrot (sort k (rots l)))).
-  Proof.
-    intros.
-    replace 1 with (Nat.min j 1) by (apply Min.min_r; omega).
-    rewrite <- cols_sort2, <- sort_succ_rrot, map_rrot_rots, cols_sort2.
-    rewrite cols_sort_perm by apply rrot_perm.
-    rewrite cols_sort2.
-    replace (Nat.min j (S k)) with (Nat.min j k) by (rewrite ?Nat.min_l; omega).
-    reflexivity.
-  Qed.
-
-  Theorem cols_id : forall n mat,
-      Forall (fun x => length x <= n) mat ->
-      cols n mat = mat.
-  Proof.
-    induction n; intros mat HL.
-    - unfold cols. unfold firstn.
-      rewrite <- map_id.
-      apply map_forall_eq.
-      eapply Forall_impl; [|apply HL].
-      simpl; intros.
-      assert (length a = 0) by omega.
-      symmetry. apply length_zero_iff_nil; auto.
-    - unfold cols. rewrite <- map_id.
-      apply map_forall_eq.
-      eapply Forall_impl; [|apply HL].
-      cbv beta. intros.
-      apply firstn_all2; auto.
-  Qed.
-End Cols.
-
-Fixpoint zipWith {A B C} (f : A -> B -> C) (a : list A) (b : list B) : list C :=
-  match (a, b) with
-  | (ahd :: atl, bhd :: btl) => f ahd bhd :: zipWith f atl btl
-  | _ => []
-  end.
-
-Section PrependColumn.
-  Context {A : Type}.
-
-  Definition prepend_col := zipWith (@cons A).
-
-  Lemma prepend_cons : forall ahd bhd atl btl,
-      prepend_col (ahd :: atl) (bhd :: btl) = (ahd :: bhd) :: prepend_col atl btl.
-  Proof. reflexivity. Qed.
-
-  Theorem prepend_hd_tl : forall l d,
-      Forall (fun x => ~ x = []) l ->
-      prepend_col (map (hd d) l) (map (@tl A) l) = l.
-  Proof.
-    induction l; intros.
-    - simpl. reflexivity.
-    - inversion H; subst; clear H.
-      cbn. rewrite IHl by auto. f_equal.
-      destruct a; try contradiction.
-      reflexivity.
-  Qed.
-
-  Lemma cols_rrot : forall j l d,
-      cols (S j) (map rrot l) = prepend_col (map (fun x => last x d) l) (cols j l).
-  Admitted.
-End PrependColumn.
-
-Section AppendCol.
-  Context {A : Type}.
-
-  Definition append_col (c : list A) (m : list (list A)) :=
-    map lrot (prepend_col c m).
-
-  Theorem map_lrot_prepend : forall c m,
-      map lrot (prepend_col c m) = append_col c m.
-  Proof.
-    reflexivity.
-  Qed.
-
-  Theorem map_rrot_append : forall c m,
-      map rrot (append_col c m) = prepend_col c m.
-  Proof.
-    intros.
-    apply map_injective with (f := lrot); [apply lrot_injective|].
-    rewrite map_map.
-    erewrite map_ext; [|apply r_l_rot_inverse].
-    rewrite map_id. reflexivity.
-  Qed.
-
-  Theorem append_last_init : forall l d,
-      Forall (fun x => ~ x = []) l ->
-      append_col (map (fun x => last x d) l) (map init l) = l.
-  Proof.
-    induction l; intros.
-    - reflexivity.
-    - inversion H; subst; clear H.
-      simpl. unfold append_col in *. cbn.
-      rewrite IHl; auto.
-      f_equal.
-      destruct a; try contradiction.
-      symmetry. apply init_last_destr.
-  Qed.
-
-  Theorem map_lrot_append : forall l d,
-      Forall (fun x => ~ x = []) l ->
-      map lrot l = append_col (map (hd d) l) (map (@tl A) l).
-  Proof.
-    intros. unfold append_col.
-    rewrite prepend_hd_tl; auto.
-  Qed.
-
-  Theorem map_rrot_prepend : forall (l : list (list A)) d,
-      Forall (fun x => ~ x = []) l ->
-      map rrot l = prepend_col (map (fun x => last x d) l) (map init l).
-  Proof.
-    intros.
-    apply map_injective with (f := lrot); [apply lrot_injective|].
-    rewrite map_map.
-    erewrite map_ext; [|apply r_l_rot_inverse].
-    rewrite map_id.
-    pose proof append_last_init as ALI.
-    unfold append_col in ALI. symmetry. auto.
-  Qed.
-End AppendCol.
-
-Section Lexsort.
-  Context {A : Type} `{Ord A}.
-
-  Lemma orig_in_sorted_rots : forall l k,
-      l <> [] -> Exists (eq l) (sort k (rots l)).
-  Proof.
-    intros.
-    apply Permutation_exists with (l0 := rots l) (l' := sort k (rots l)).
-    apply sort_perm.
-    apply orig_in_rots. auto.
-  Qed.
-
-  Lemma sort_rots_len : forall k l,
-      Forall (fun x => length x = length l) (sort k (rots l)).
-  Proof.
-    intros.
-    eapply Permutation_forall.
-    apply sort_perm. apply rots_row_length.
-  Qed.
-End Lexsort.
-
-Section FindIndex.
-  Context {A : Type} `{EqDec A}.
-
-  Fixpoint findIndex (x : A) (ls : list A) : nat :=
-    match ls with
-    | [] => 0
-    | hd :: tl =>
-      match x == hd with
-      | left _ => 0
-      | right Neq => S (findIndex x tl)
-      end
+    match l with
+    | [] => []
+    | hd :: tl => List.map (fun x => last x hd) (sort (length l) (rots l))
     end.
-
-  Theorem findIndex_correct : forall x xs d,
-      Exists (equiv x) xs -> nth (findIndex x xs) xs d === x.
-  Proof.
-    intros x xs d E.
-    unfold findIndex.
-    induction E.
-    - destruct (x == x0).
-      + simpl. apply equiv_symmetric. auto.
-      + contradiction.
-    - destruct (x == x0).
-      + simpl. apply equiv_symmetric. auto.
-      + apply IHE.
-  Qed.
-
-  Theorem findIndex_bounds : forall x xs,
-      Exists (equiv x) xs -> findIndex x xs < length xs.
-  Proof.
-    intros x xs E.
-    unfold findIndex.
-    induction E.
-    - destruct (x == x0).
-      + simpl. apply Nat.lt_0_succ.
-      + contradiction.
-    - destruct (x == x0).
-      + simpl. apply Nat.lt_0_succ.
-      + simpl. apply le_n_S. apply IHE.
-  Qed.
-End FindIndex.
 
 Section Transform.
   Context {A : Type} `{O: Ord A} `{E : EqDec A eq}.
@@ -416,75 +74,79 @@ Section Transform.
   Qed.
 
   Definition bwn (l : list A) : nat :=
-    findIndex l (sort (length l) (rots l)).
+    findIx l (sort (length l) (rots l)).
 
   Theorem bwn_correct : forall xs d,
     xs <> [] -> nth (bwn xs) (sort (length xs) (rots xs)) d = xs.
   Proof.
     intros.
     unfold bwn.
-    apply findIndex_correct.
+    apply findIx_correct.
     apply orig_in_sorted_rots. auto.
   Qed.
 End Transform.
 
-Lemma map_const {A B} : forall (f : A -> B) l c,
-    (forall x, f x = c) -> map f l = repeat c (length l).
-Proof.
-  intros.
-  induction l; [reflexivity|].
-  simpl. rewrite H. f_equal. auto.
-Qed.
+Section ReverseTransform.
+  Section Recreate.
+    Context {A : Type} `{Ord A}.
 
-Section Recreate.
-  Context {A : Type} `{Ord A}.
+    Fixpoint recreate (j : nat) (l : list A) : list (list A) :=
+      match j with
+      | O    => map (const []) l
+      | S j' => sort 1 (prepend_col l (recreate j' l))
+      end.
 
-  Fixpoint recreate (j : nat) (l : list A) : list (list A) :=
-    match j with
-    | O    => map (const []) l
-    | S j' => sort 1 (prepend_col l (recreate j' l))
-    end.
-
-  Theorem recreate_inspiration : forall j l,
-      j < length l ->
-      cols (S j) (sort (length l) (rots l)) =
-      sort 1 (prepend_col (bwp l) (cols j (sort (length l) (rots l)))).
-  Proof.
-    intros. destruct l eqn:HL; [reflexivity|].
-    rewrite <- HL in *. assert (l <> []) by (intro c; subst; inversion c).
-    rewrite cols_sort_shift by omega.
-    rewrite cols_rrot with (d := a).
-    rewrite <- bwp_nonempty with (d := a) by auto.
-    reflexivity.
-  Qed.
-
-  Lemma recreate_correct_gen : forall j l,
-      j <= length l ->
-      recreate j (bwp l) = cols j (sort (length l) (rots l)).
-  Proof.
-    induction j; intros.
-    - unfold cols. simpl.
-      do 2 (erewrite map_const; [|unfold const; reflexivity]).
-      rewrite bwp_length, sort_length, rots_length.
+    Theorem recreate_inspiration : forall j l,
+        j < length l ->
+        cols (S j) (sort (length l) (rots l)) =
+        sort 1 (prepend_col (bwp l) (cols j (sort (length l) (rots l)))).
+    Proof.
+      intros. destruct l eqn:HL; [reflexivity|].
+      rewrite <- HL in *. assert (l <> []) by (intro c; subst; inversion c).
+      rewrite cols_sort_shift by omega.
+      rewrite cols_rrot with (d := a).
+      rewrite <- bwp_nonempty with (d := a) by auto.
       reflexivity.
-    - simpl.
-      rewrite recreate_inspiration by omega.
-      rewrite IHj by omega.
-      reflexivity.
-  Qed.
+    Qed.
 
-  Theorem recreate_correct : forall l,
-      recreate (length l) (bwp l) = sort (length l) (rots l).
-  Proof.
-    intros.
-    rewrite recreate_correct_gen by omega.
-    rewrite cols_id; auto.
-    eapply Forall_impl; [|apply sort_rots_len].
-    cbv beta; intros; omega.
-  Qed.
-End Recreate.
+    Lemma recreate_correct_gen : forall j l,
+        j <= length l ->
+        recreate j (bwp l) = cols j (sort (length l) (rots l)).
+    Proof.
+      induction j; intros.
+      - unfold cols.
+        erewrite map_const with (g := const []) (ys := bwp l);
+          [| |rewrite bwp_length, sort_length, rots_length]; [|reflexivity..].
+        reflexivity.
+      - assert (rrot_hdsort_id : forall xs,
+                   sort (length xs) (rots xs) =
+                   sort 1 (map rrot (sort (length xs) (rots xs)))) by admit.
+        rewrite rrot_hdsort_id.
+        assert (cols_hdsort_comm : forall j xs,
+                   cols (S j) (sort 1 xs) =
+                   sort 1 (cols (S j) xs)) by admit.
+        rewrite cols_hdsort_comm.
+        rewrite cols_rrot.
+        assert (cols_succ_rrot : forall j xs d,
+                   cols (S j) (map rrot xs) =
+                   prepend_col (map (fun l => last l d) xs) (cols j xs)).
+        simpl.
+        rewrite recreate_inspiration by omega.
+        rewrite IHj by omega.
+        reflexivity.
+    Qed.
 
-Section Unbwt.
+    Theorem recreate_correct : forall l,
+        recreate (length l) (bwp l) = sort (length l) (rots l).
+    Proof.
+      intros.
+      rewrite recreate_correct_gen by omega.
+      rewrite cols_id; auto.
+      eapply Forall_impl; [|apply sort_rots_len].
+      cbv beta; intros; omega.
+    Qed.
+  End Recreate.
+
   Context {A : Type} `{O : Ord A} `{E : EqDec A eq}.
 
   Definition unbwt (t : nat) (l : list A) : list A :=
@@ -500,4 +162,4 @@ Section Unbwt.
     apply bwn_correct.
     intro contra; inversion contra.
   Qed.
-End Unbwt.
+End ReverseTransform.
