theories/BWT/FindIx.v
@@ -1,0 +1,47 @@
+Require Import Coq.Classes.EquivDec.
+Require Import Coq.Lists.List.
+Require Import Coq.Arith.PeanoNat.
+
+Import ListNotations.
+
+Section FindIx.
+  Context {A : Type} `{EqDec A}.
+
+  Fixpoint findIx (x : A) (ls : list A) : nat :=
+    match ls with
+    | [] => 0
+    | hd :: tl =>
+      match x == hd with
+      | left _ => 0
+      | right Neq => S (findIx x tl)
+      end
+    end.
+
+  Theorem findIx_correct : forall x xs d,
+      Exists (equiv x) xs -> nth (findIx x xs) xs d === x.
+  Proof.
+    intros x xs d E.
+    unfold findIx.
+    induction E.
+    - destruct (x == x0).
+      + simpl. apply equiv_symmetric. auto.
+      + contradiction.
+    - destruct (x == x0).
+      + simpl. apply equiv_symmetric. auto.
+      + apply IHE.
+  Qed.
+
+  Theorem findIx_bounds : forall x xs,
+      Exists (equiv x) xs -> findIx x xs < length xs.
+  Proof.
+    intros x xs E.
+    unfold findIx.
+    induction E.
+    - destruct (x == x0).
+      + simpl. apply Nat.lt_0_succ.
+      + contradiction.
+    - destruct (x == x0).
+      + simpl. apply Nat.lt_0_succ.
+      + simpl. apply le_n_S. apply IHE.
+  Qed.
+End FindIx.
