theories/BWT/Lib.v
@@ -1,0 +1,115 @@
+Require Import Coq.Lists.List.
+Require Import Coq.Program.Basics.
+Require Import Coq.omega.Omega.
+
+Open Scope program_scope.
+
+Section Forall2.
+  Lemma Forall2_eq {A : Type} : forall x y : list A,
+    Forall2 eq x y <-> x = y.
+  Proof.
+    split; intros.
+    - induction H.
+      + reflexivity.
+      + subst. f_equal.
+    - subst. induction y; constructor; auto.
+  Qed.
+
+  Lemma Forall2_map {A B : Type} (R : B -> B -> Prop) : forall (f : A -> B) (l l' : list A),
+      length l = length l' ->
+      Forall2 R (map f l) (map f l') <-> Forall2 (fun x y => R (f x) (f y)) l l'.
+  Proof.
+    induction l; intros.
+    - simpl in H.
+      replace l' with (@nil A) by (symmetry; apply length_zero_iff_nil; auto).
+      split; constructor.
+    - destruct l' as [|a' l']; [inversion H|].
+      simpl; split; intros HImp; inversion HImp; subst; clear HImp; constructor; auto.
+      + apply IHl; auto.
+      + apply IHl; auto.
+  Qed.
+
+  Lemma Forall2_impl : forall (A B : Type) (P Q : A -> B -> Prop),
+      (forall a b, P a b -> Q a b) -> forall l l', Forall2 P l l' -> Forall2 Q l l'.
+  Proof.
+    intros. induction H0; constructor; auto.
+  Qed.
+End Forall2.
+
+Section Map.
+  Lemma eq_map {A B : Type} (f g : A -> B) l :
+    (forall x, f x = g x) -> map f l = map g l.
+  Proof.
+    intros HExt; induction l; try reflexivity.
+    simpl; rewrite HExt, IHl.
+    reflexivity.
+  Qed.
+
+  Lemma map_map' {A B C : Type} : forall (f : A -> B) (g : B -> C) l,
+      map g (map f l) = map (g ∘ f) l.
+  Proof.
+    intros.
+    rewrite map_map. apply eq_map.
+    reflexivity.
+  Qed.
+
+  Lemma map_injective {A B : Type} : forall (f : A -> B) l l',
+      (forall x y, f x = f y -> x = y) ->
+      map f l = map f l' -> l = l'.
+  Proof.
+    intros f l l' HInj MapEq.
+    assert (length l = length l'). {
+      rewrite <- map_length with (f := f), MapEq, -> map_length.
+      easy.
+    }
+    assert (Forall2 (fun x y => f x = f y) l l'). {
+      apply Forall2_eq in MapEq.
+      apply (proj1 (Forall2_map eq f l l' H)) in MapEq.
+      apply MapEq.
+    }
+    apply Forall2_eq.
+    eapply Forall2_impl; [| apply H0].
+    cbv beta; intros. auto.
+  Qed.
+
+  Lemma map_forall_eq {A B : Type} : forall (l : list A) (f g : A -> B),
+      Forall (fun x => f x = g x) l -> map f l = map g l.
+  Proof.
+    induction l; intros.
+    - reflexivity.
+    - inversion H; subst; clear H.
+      simpl. f_equal; auto.
+  Qed.
+
+  Lemma map_const_repeat {A B} : forall (f : A -> B) l c,
+      (forall x, f x = c) -> map f l = repeat c (length l).
+  Proof.
+    intros.
+    induction l; [reflexivity|].
+    simpl. rewrite H. f_equal. auto.
+  Qed.
+
+  Lemma const_const {A} : forall c x y : A,
+      const c x = const c y.
+  Proof. reflexivity. Qed.
+
+  Lemma map_const {A B C} : forall (f : A -> C) (g : B -> C),
+      (forall x y, f x = g y) ->
+      forall xs ys,
+        length xs = length ys ->
+        map f xs = map g ys.
+  Proof.
+    intros f g Hconst xs ys HL.
+    destruct (length xs) eqn:Hn.
+    - replace xs with (@nil A); replace ys with (@nil B);
+        [reflexivity|symmetry; apply length_zero_iff_nil; omega..].
+    - destruct xs as [|a xtl] eqn:Hxs; [cbn in Hn; omega|].
+      destruct ys as [|b ytl] eqn:Hys; [cbn in Hn, HL; omega|].
+      rewrite <- Hxs, <- Hys, <- Hn in *; clear Hn Hxs Hys xtl ytl.
+      rewrite map_const_repeat with (c := f a)
+        by (rewrite Hconst with (y := b); easy).
+      rewrite map_const_repeat with (c := g b)
+        by (rewrite <- Hconst with (x := a); easy).
+      f_equal; auto.
+  Qed.
+End Map.
