theories/BWT/Matrix.v
@@ -1,0 +1,209 @@
+Require Import BWT.Sorting.Ord.
+Require Import Coq.Program.Basics.
+Require Import Coq.Lists.List.
+Require Import BWT.Sorting.Prefix.
+Require Import BWT.Rotation.
+Require Import BWT.Repeat.
+Require Import BWT.Lib.
+Require Import BWT.Rots.
+Require Import Coq.Arith.PeanoNat.
+Require Import Coq.Sorting.Permutation.
+Require Import Coq.omega.Omega.
+
+Import ListNotations.
+
+Open Scope program_scope.
+
+Section SortRotations.
+  Context {A : Type} `{O : Ord A}.
+
+  Theorem foo : forall k l,
+sort (S k) (map rrot l) = (sort 1 ∘ map rrot) (sort k l) ->
+      @sort A O (S k) (map rrot l) = @sort A O 1 (map rrot (sort k l)).
+  Proof. unfold compose in *. easy. Qed.
+
+  Lemma sort_succ_k : forall k l,
+      sort (S k) l = sort 1 (map rrot (sort k (map lrot l))).
+  Proof.
+  Admitted.
+
+  Theorem sort_rrot_k : forall k l,
+    sort k (map (rep rrot k) l)= rep (sort 1 ∘ map rrot) k l.
+  Proof.
+  Admitted.
+
+  Lemma sort_succ_rrot : forall k (l : list (list A)),
+      @sort A O (S k) (map rrot l) = @sort A O 1 (map rrot (sort k l)).
+  Proof.
+    intros.
+    pose proof (sort_rrot_k (S k)) as E6.
+    simpl rep at 2 in E6.
+    specialize E6 with (l := map (rep lrot k) l).
+    rewrite <- sort_rrot_k in E6.
+    pose proof rep_inv_r (@lrot A) rrot l_r_rot_inverse as rep_inv.
+    do 2 rewrite map_map' in E6.
+    rewrite eq_map with (f := rep rrot (S k) ∘ rep lrot k) (g := rrot) in E6
+      by (intros; unfold compose;
+          rewrite rep_inv, Nat.sub_succ_l, Nat.sub_diag;
+          [reflexivity|apply Nat.le_refl|apply Nat.le_succ_diag_r]).
+    rewrite eq_map with (f := rep rrot k ∘ rep lrot k) (g := id)in E6
+      by (intros; unfold compose; rewrite rep_inv;
+          [rewrite Nat.sub_diag; reflexivity|apply Nat.le_refl]).
+    (* TODO For some reason hangs at the end *)
+    replace (sort 1 (map rrot (sort k l)))
+    with ((sort 1 ∘ map rrot) (sort k l)) by reflexivity.
+    rewrite map_id in E6.
+    apply E6.
+  Qed.
+
+End SortRotations.
+
+Section Cols.
+  Context {A : Type}.
+
+  Definition cols j := map (@firstn A j).
+
+  Context `{Ord A}.
+
+  Theorem cols_sort1 : forall k j l,
+      cols j (sort k l) = cols j (sort (Nat.min j k) l).
+  Admitted.
+
+  Theorem cols_sort2 : forall k j l,
+      cols j (sort k l) = sort (Nat.min j k) (cols j l).
+  Admitted.
+
+  Lemma cols_sort_lt : forall k j l,
+      j <= k -> cols j (sort k l) = sort j (cols j l).
+  Proof.
+    intros.
+    replace j with (Nat.min j k) at 2 by (apply Min.min_l; auto).
+    apply cols_sort2.
+  Qed.
+
+  Theorem cols_sort_perm : forall k j p l,
+      (forall l, Permutation l (p l)) -> cols j (sort k (p l)) = cols j (sort k l).
+  Admitted.
+
+  Theorem cols_sort_shift : forall k j l,
+      1 <= j <= k ->
+      cols j (sort k (rots l)) = sort 1 (cols j (map rrot (sort k (rots l)))).
+  Proof.
+    intros.
+    replace 1 with (Nat.min j 1) by (apply Min.min_r; omega).
+    rewrite <- cols_sort2, <- sort_succ_rrot, map_rrot_rots, cols_sort2.
+    rewrite cols_sort_perm by apply rrot_perm.
+    rewrite cols_sort2.
+    replace (Nat.min j (S k)) with (Nat.min j k) by (rewrite ?Nat.min_l; omega).
+    reflexivity.
+  Qed.
+
+  Theorem cols_id : forall n mat,
+      Forall (fun x => length x <= n) mat ->
+      cols n mat = mat.
+  Proof.
+    induction n; intros mat HL.
+    - unfold cols. unfold firstn.
+      rewrite <- map_id.
+      apply map_forall_eq.
+      eapply Forall_impl; [|apply HL].
+      simpl; intros.
+      assert (length a = 0) by omega.
+      symmetry. apply length_zero_iff_nil; auto.
+    - unfold cols. rewrite <- map_id.
+      apply map_forall_eq.
+      eapply Forall_impl; [|apply HL].
+      cbv beta. intros.
+      apply firstn_all2; auto.
+  Qed.
+End Cols.
+
+Fixpoint zipWith {A B C} (f : A -> B -> C) (a : list A) (b : list B) : list C :=
+  match (a, b) with
+  | (ahd :: atl, bhd :: btl) => f ahd bhd :: zipWith f atl btl
+  | _ => []
+  end.
+
+Section PrependColumn.
+  Context {A : Type}.
+
+  Definition prepend_col := zipWith (@cons A).
+
+  Lemma prepend_cons : forall ahd bhd atl btl,
+      prepend_col (ahd :: atl) (bhd :: btl) = (ahd :: bhd) :: prepend_col atl btl.
+  Proof. reflexivity. Qed.
+
+  Theorem prepend_hd_tl : forall l d,
+      Forall (fun x => ~ x = []) l ->
+      prepend_col (map (hd d) l) (map (@tl A) l) = l.
+  Proof.
+    induction l; intros.
+    - simpl. reflexivity.
+    - inversion H; subst; clear H.
+      cbn. rewrite IHl by auto. f_equal.
+      destruct a; try contradiction.
+      reflexivity.
+  Qed.
+
+  Lemma cols_rrot : forall j l d,
+      cols (S j) (map rrot l) = prepend_col (map (fun x => last x d) l) (cols j l).
+  Admitted.
+End PrependColumn.
+
+Section AppendCol.
+  Context {A : Type}.
+
+  Definition append_col (c : list A) (m : list (list A)) :=
+    map lrot (prepend_col c m).
+
+  Theorem map_lrot_prepend : forall c m,
+      map lrot (prepend_col c m) = append_col c m.
+  Proof.
+    reflexivity.
+  Qed.
+
+  Theorem map_rrot_append : forall c m,
+      map rrot (append_col c m) = prepend_col c m.
+  Proof.
+    intros.
+    apply map_injective with (f := lrot); [apply lrot_injective|].
+    rewrite map_map.
+    erewrite map_ext; [|apply r_l_rot_inverse].
+    rewrite map_id. reflexivity.
+  Qed.
+
+  Theorem append_last_init : forall l d,
+      Forall (fun x => ~ x = []) l ->
+      append_col (map (fun x => last x d) l) (map init l) = l.
+  Proof.
+    induction l; intros.
+    - reflexivity.
+    - inversion H; subst; clear H.
+      simpl. unfold append_col in *. cbn.
+      rewrite IHl; auto.
+      f_equal.
+      destruct a; try contradiction.
+      symmetry. apply init_last_destr.
+  Qed.
+
+  Theorem map_lrot_append : forall l d,
+      Forall (fun x => ~ x = []) l ->
+      map lrot l = append_col (map (hd d) l) (map (@tl A) l).
+  Proof.
+    intros. unfold append_col.
+    rewrite prepend_hd_tl; auto.
+  Qed.
+
+  Theorem map_rrot_prepend : forall (l : list (list A)) d,
+      Forall (fun x => ~ x = []) l ->
+      map rrot l = prepend_col (map (fun x => last x d) l) (map init l).
+  Proof.
+    intros.
+    apply map_injective with (f := lrot); [apply lrot_injective|].
+    rewrite map_map.
+    erewrite map_ext; [|apply r_l_rot_inverse].
+    rewrite map_id.
+    pose proof append_last_init as ALI.
+    unfold append_col in ALI. symmetry. auto.
+  Qed.
+End AppendCol.
