theories/BWT/NonEmptyList.v
@@ -1,0 +1,168 @@
+Require Import Coq.omega.Omega.
+Require Coq.Lists.List.
+Require Import Coq.Program.Wf.
+
+Import List.ListNotations.
+Bind Scope list_scope with List.list.
+
+Inductive list (A : Type) : Type :=
+| wrap : A -> list A
+| cons : A -> list A -> list A.
+
+Arguments wrap {_}.
+Arguments cons {_}.
+
+Infix "::" := cons (at level 60, right associativity) : ne_list_scope.
+Delimit Scope ne_list_scope with ne_list.
+Bind Scope ne_list_scope with list.
+
+Fixpoint ne_cons {A} (x : A) (xs : List.list A) : list A :=
+  match xs with
+  | []%list => wrap x
+  | (hd :: tl)%list => x :: ne_cons hd tl
+  end.
+
+Module ListNotations.
+  Notation "[ x ]" := (wrap x) : ne_list_scope.
+  Notation "[ x ; y ]" := (cons x (wrap y)) : ne_list_scope.
+  Notation "[ w ; x ; y ; .. ; z ]" := (ne_cons w (List.cons x (List.cons y .. (List.cons z List.nil) .. ))) : ne_list_scope.
+End ListNotations.
+
+Import ListNotations.
+Open Scope ne_list_scope.
+
+Fixpoint snoc {A} (x : A) (xs : list A) : list A :=
+  match xs with
+  | [y] => y :: [x]
+  | hd :: tl => hd :: snoc x tl
+  end.
+
+Fixpoint ne_snoc {A} (x : A) (xs : List.list A) : list A :=
+  match xs with
+  | []%list => wrap x
+  | (hd :: tl)%list => hd :: ne_snoc x tl
+  end.
+
+Program Fixpoint embed {A} (xs : list A) : { xs : List.list A | xs <> List.nil } :=
+  match xs with
+  | [x] => [x]%list
+  | hd :: tl => (hd :: embed tl)%list
+  end.
+
+Program Fixpoint extract {A} (xs: { xs : List.list A | xs <> List.nil })
+        {measure (length xs)}
+  : list A
+  :=
+  match xs with
+  | []%list => _
+  | [x]%list => [x]
+  | (hd :: tl)%list => hd :: extract tl
+  end.
+Next Obligation.
+  specialize (H hd).
+  intro contra. rewrite contra in H.
+  contradiction H. easy.
+Defined.
+
+Theorem ne_cons_correct {A} : forall xs (x : A),
+    embed (ne_cons x xs) = (x :: xs)%list.
+Proof. induction xs; simpl; [|rewrite IHxs]; reflexivity. Qed.
+
+Theorem ne_snoc_correct {A} : forall xs (x : A),
+    embed (ne_snoc x xs) = (xs ++ [x])%list.
+Proof. induction xs; intros; simpl; [|rewrite <- IHxs]; reflexivity. Qed.
+
+Definition head {A} (xs : list A) : A :=
+  match xs with
+  | [x] => x
+  | x :: _ => x
+  end.
+
+Definition tail {A} (xs : list A) : List.list A :=
+  match xs with
+  | [_] => List.nil
+  | _ :: tl => embed tl
+  end.
+
+Fixpoint last {A} (xs : list A) : A :=
+  match xs with
+  | [x] => x
+  | _ :: tl => last tl
+  end.
+
+Fixpoint init {A} (xs : list A) : List.list A :=
+  match xs with
+  | [_] => List.nil
+  | hd :: tl => hd :: init tl
+  end.
+
+Theorem head_cons {A} : forall (hd : A) tl,
+    head (hd :: tl) = hd.
+Proof. reflexivity. Qed.
+
+Theorem tail_cons {A} : forall (hd : A) tl,
+    tail (hd :: tl) = embed tl.
+Proof. reflexivity. Qed.
+
+Theorem head_tail_id {A} : forall xs : list A,
+    ne_cons (head xs) (tail xs) = xs.
+Proof.
+  induction xs; [reflexivity|].
+  cbn. rewrite <- IHxs.
+  rewrite ne_cons_correct. reflexivity.
+Qed.
+
+Theorem head_ne_cons {A} : forall (hd : A) tl,
+    head (ne_cons hd tl) = hd.
+Proof. destruct tl; reflexivity. Qed.
+
+Theorem tail_ne_cons {A} : forall (hd : A) tl,
+    tail (ne_cons hd tl) = tl.
+Proof. destruct tl; [reflexivity|apply ne_cons_correct]. Qed.
+
+Theorem last_snoc {A} : forall (lt : A) it,
+    last (snoc lt it) = lt.
+Proof. induction it; auto. Qed.
+
+Theorem init_snoc {A} : forall (lt : A) it,
+    init (snoc lt it) = embed it.
+Proof. induction it; cbn; [|rewrite IHit]; easy. Qed.
+
+Theorem last_ne_snoc {A} : forall (lt : A) it,
+    last (ne_snoc lt it) = lt.
+Proof. induction it; cbn; [|rewrite IHit]; easy. Qed.
+
+Theorem init_ne_snoc {A} : forall (lt : A) it,
+    init (ne_snoc lt it) = it.
+Proof. induction it; cbn; [|rewrite IHit]; easy. Qed.
+
+Theorem last_init_id {A} : forall xs : list A,
+    ne_snoc (last xs) (init xs) = xs.
+Proof.
+  induction xs; [reflexivity|].
+  cbn. rewrite IHxs. reflexivity.
+Qed.
+
+Fixpoint length {A} (xs : list A) : nat :=
+  match xs with
+  | [_] => 1
+  | _ :: tl => S (length tl)
+  end.
+
+Theorem length_gt_zero {A} : forall xs : list A,
+    length xs > 0.
+Proof. induction xs; cbn; omega. Qed.
+
+Theorem length_correct {A} : forall xs : list A,
+    length xs = List.length (embed xs).
+Proof. induction xs; cbn; auto. Qed.
+
+Fixpoint map {A B} (f : A -> B) (xs : list A) : list B :=
+  match xs with
+  | [x] => [f x]
+  | hd :: tl => f hd :: map f tl
+  end.
+
+Theorem map_correct {A B} : forall (f : A -> B) xs,
+    embed (map f xs) = List.map f (embed xs).
+Proof. induction xs; cbn; [|rewrite IHxs]; easy. Qed.
